Simplify type environments

formalization/Psamathe.thy
@@ -3,40 +3,41 @@ theory Psamathe
 begin
 
 datatype TyQuant = empty | any | one | nonempty
-datatype BaseTy = nat
+datatype BaseTy = natural | boolean
 type_synonym Type = "TyQuant \<times> BaseTy"
 datatype Mode = s | d
-datatype Locator = C nat | V string 
+datatype Locator = N nat | B bool | V string 
                  | VDef string BaseTy ("var _ : _")
 datatype Stmt = Flow Locator Locator
 datatype Prog = Prog "Stmt list"
 
-type_synonym Env = "(string \<times> Type) set"
+type_synonym Env = "(string, Type) map"
 
 definition toQuant :: "nat \<Rightarrow> TyQuant" where
   "toQuant n \<equiv> (if n = 0 then empty else if n = 1 then one else nonempty)"
-definition dom :: "Env \<Rightarrow> string set" where
-  "dom \<Gamma> \<equiv> { x . \<exists>\<tau>. (x,\<tau>) \<in> \<Gamma> }"
 
 inductive loc_type :: "Env \<Rightarrow> Mode \<Rightarrow> Locator \<Rightarrow> Type \<Rightarrow> (Type \<Rightarrow> Type) \<Rightarrow> Env \<Rightarrow> bool"
   ("_ \<turnstile>{_} _ : _ ; _ \<stileturn> _") where
-  Nat: "\<Gamma> \<turnstile>{s} (C n) : (toQuant(n), nat) ; f \<stileturn> \<Gamma>"
-| Var: "(\<Gamma> \<union> {(x, \<tau>)}) \<turnstile>{m} (V x) : \<tau> ; f \<stileturn> (\<Gamma> \<union> {(x, f(\<tau>))})"
-| VarDef: "\<lbrakk> x \<notin> dom \<Gamma> \<rbrakk> \<Longrightarrow> \<Gamma> \<turnstile>{d} (var x : t) : (empty, t) ; f \<stileturn> (\<Gamma> \<union> {(x, f(empty, t))})"
+  Nat: "\<Gamma> \<turnstile>{s} (N n) : (toQuant(n), natural) ; f \<stileturn> \<Gamma>"
+| Bool: "\<Gamma> \<turnstile>{s} (B b) : (one, boolean) ; f \<stileturn> \<Gamma>"
+| Var: "\<lbrakk> \<Gamma> x = Some \<tau> \<rbrakk> \<Longrightarrow> \<Gamma> \<turnstile>{m} (V x) : \<tau> ; f \<stileturn> (\<Gamma>(x \<mapsto> f(\<tau>)))"
+| VarDef: "\<lbrakk> x \<notin> dom \<Gamma> \<rbrakk> \<Longrightarrow> \<Gamma> \<turnstile>{d} (var x : t) : (empty, t) ; f \<stileturn> (\<Gamma>(x \<mapsto> f(empty, t)))"
 
-datatype Val = Num nat | error
+datatype Val = Num nat | Bool bool | error
 datatype Loc = SLoc nat | Amount nat
 type_synonym Resource = "BaseTy \<times> Val"
 type_synonym Store = "(string, nat \<times> Loc) map \<times> (nat, Resource) map"
 
 fun emptyVal :: "BaseTy \<Rightarrow> Val" where
-  "emptyVal nat = Num 0"
+  "emptyVal natural = Num 0"
+| "emptyVal boolean = Bool False"
 
 inductive loc_eval :: "Store \<Rightarrow> Locator \<Rightarrow> Store \<Rightarrow> (Locator + Loc \<times> Loc) \<Rightarrow> bool"
   ("< _ , _ > \<rightarrow> < _ , _ >") where
-  ENat: "\<lbrakk> l \<notin> Map.dom \<rho> \<rbrakk> \<Longrightarrow> < (\<mu>, \<rho>), C n > \<rightarrow> < (\<mu>, \<rho>(l \<mapsto> (nat, Num n))), Inr (SLoc l, Amount n) >"
+  ENat: "\<lbrakk> l \<notin> dom \<rho> \<rbrakk> \<Longrightarrow> < (\<mu>, \<rho>), N n > \<rightarrow> < (\<mu>, \<rho>(l \<mapsto> (natural, Num n))), Inr (SLoc l, Amount n) >"
+| EBool: "\<lbrakk> l \<notin> dom \<rho> \<rbrakk> \<Longrightarrow> < (\<mu>, \<rho>), B b > \<rightarrow> < (\<mu>, \<rho>(l \<mapsto> (boolean, Bool b))), Inr (SLoc l, SLoc l) >"
 | EVar: "\<lbrakk> \<mu> x = Some (l, k) \<rbrakk> \<Longrightarrow> < (\<mu>, \<rho>), V x > \<rightarrow> < (\<mu>, \<rho>), Inr (SLoc l, k) >"
-| EVarDef: "\<lbrakk> x \<notin> Map.dom \<mu> ; l \<notin> Map.dom \<rho> \<rbrakk> 
+| EVarDef: "\<lbrakk> x \<notin> dom \<mu> ; l \<notin> dom \<rho> \<rbrakk> 
             \<Longrightarrow> < (\<mu>, \<rho>), var x : t > 
                 \<rightarrow> < (\<mu>(x \<mapsto> (l, SLoc l)), \<rho>(l \<mapsto> (t, emptyVal t))), Inr (SLoc l, SLoc l) >"
 
@@ -53,9 +54,6 @@ fun compat :: "Env \<Rightarrow> Store \<Rightarrow> bool" ("_ \<leftrightarrow>
   "compat \<Gamma> (\<mu>, \<rho>) = ((dom \<Gamma> = Map.dom \<mu>) \<and> 
                       (\<forall>x l k. \<mu> x = Some (l, k) \<longrightarrow> \<rho> l \<noteq> None))"
 
-lemma dom_insert[simp]: "dom (insert (x, \<tau>) \<Gamma>) = insert x (dom \<Gamma>)"
-  by (cases "\<tau>", auto simp: dom_def)
-
 lemma
   fixes "\<Gamma>" and "\<L>" and "q" and "t" and "\<Delta>" and "\<mu>" and "\<rho>" and "l"
   assumes "\<Gamma> \<turnstile>{s} \<L> : (q,t) ; (\<lambda>(_, t'). (empty, t')) \<stileturn> \<Delta>"
@@ -69,34 +67,46 @@ proof(induction rule: loc_type.induct)
         and has_loc: "l \<notin> Map.dom \<rho>" by auto
   then show ?case
   proof - 
-    show "\<exists>\<mu>'. \<exists>\<rho>'. \<exists>\<L>'. (\<Gamma> \<leftrightarrow> (\<mu>', \<rho>')) \<and> < (\<mu>, \<rho>), C n > \<rightarrow> < (\<mu>', \<rho>'), \<L>' >" 
+    show "\<exists>\<mu>'. \<exists>\<rho>'. \<exists>\<L>'. (\<Gamma> \<leftrightarrow> (\<mu>', \<rho>')) \<and> < (\<mu>, \<rho>), N n > \<rightarrow> < (\<mu>', \<rho>'), \<L>' >" 
     proof(rule exI[where x = "\<mu>"], 
-          rule exI[where x = "\<rho>(l \<mapsto> (nat, Num n))"], 
+          rule exI[where x = "\<rho>(l \<mapsto> (natural, Num n))"], 
           rule exI[where x = "Inr (SLoc l, Amount n)"],
           rule conjI)
-      from env_compat show "\<Gamma> \<leftrightarrow> (\<mu>, \<rho>(l \<mapsto> (BaseTy.nat, Num n)))" by auto
-      from has_loc show " < (\<mu>, \<rho>) , C n > \<rightarrow> < (\<mu>, \<rho>(l \<mapsto> (BaseTy.nat, Num n))) , Inr (SLoc l, Amount n) >"
+      from env_compat show "\<Gamma> \<leftrightarrow> (\<mu>, \<rho>(l \<mapsto> (natural, Num n)))" by auto
+      from has_loc show " < (\<mu>, \<rho>) , N n > \<rightarrow> < (\<mu>, \<rho>(l \<mapsto> (natural, Num n))) , Inr (SLoc l, Amount n) >"
         by (rule ENat)
     qed
   qed
 next
-  case (Var \<Gamma> x \<tau> m f)
-  then have env_compat: "(\<Gamma> \<union> {(x, \<tau>)}) \<leftrightarrow> (\<mu>, \<rho>)" by auto
-  then have "x \<in> Map.dom \<mu>" 
-  proof -
-    have in_type_env: "x \<in> dom (\<Gamma> \<union> {(x, \<tau>)})" 
-      by (simp only: dom_def Set.mem_Collect_eq, rule exI[where x = "\<tau>"], auto)
-    from this and env_compat show "x \<in> Map.dom \<mu>" by auto
+  case (Bool \<Gamma> b f)
+  then have env_compat: "\<Gamma> \<leftrightarrow> (\<mu>, \<rho>)" 
+        and has_loc: "l \<notin> Map.dom \<rho>" by auto
+  then show ?case
+  proof - 
+    show "\<exists>\<mu>'. \<exists>\<rho>'. \<exists>\<L>'. (\<Gamma> \<leftrightarrow> (\<mu>', \<rho>')) \<and> < (\<mu>, \<rho>), B b > \<rightarrow> < (\<mu>', \<rho>'), \<L>' >" 
+    proof(rule exI[where x = "\<mu>"], 
+          rule exI[where x = "\<rho>(l \<mapsto> (boolean, Bool b))"], 
+          rule exI[where x = "Inr (SLoc l, SLoc l)"],
+          rule conjI)
+      from env_compat show "\<Gamma> \<leftrightarrow> (\<mu>, \<rho>(l \<mapsto> (boolean, Bool b)))" by auto
+      from has_loc show " < (\<mu>, \<rho>) , B b > \<rightarrow> < (\<mu>, \<rho>(l \<mapsto> (boolean, Bool b))) , Inr (SLoc l, SLoc l) >"
+        by (rule EBool)
+    qed
   qed
+next
+  case (Var \<Gamma> x \<tau> m f)
+  then have env_compat: "\<Gamma> \<leftrightarrow> (\<mu>, \<rho>)"
+        and x_in_env: "\<Gamma> x = Some \<tau>" by auto
+  then have "x \<in> Map.dom \<mu>" by auto
   then obtain xl and k where in_lookup: "\<mu> x = Some (xl, k)" by auto
   then show ?case
   proof -
-    show "\<exists>\<mu>'. \<exists>\<rho>'. \<exists>\<L>'. ((\<Gamma> \<union> {(x, f \<tau>)}) \<leftrightarrow> (\<mu>', \<rho>')) \<and> < (\<mu>, \<rho>) , V x > \<rightarrow> < (\<mu>', \<rho>') , \<L>' >"
+    show "\<exists>\<mu>'. \<exists>\<rho>'. \<exists>\<L>'. (\<Gamma>(x \<mapsto> f(\<tau>)) \<leftrightarrow> (\<mu>', \<rho>')) \<and> < (\<mu>, \<rho>) , V x > \<rightarrow> < (\<mu>', \<rho>') , \<L>' >"
     proof(rule exI[where x = "\<mu>"],
           rule exI[where x = "\<rho>"],
           rule exI[where x = "Inr (SLoc xl, k)"],
           rule conjI)
-      from env_compat show "(\<Gamma> \<union> {(x, f \<tau>)}) \<leftrightarrow> (\<mu>, \<rho>)" by simp
+      from env_compat and x_in_env show "\<Gamma>(x \<mapsto> f(\<tau>)) \<leftrightarrow> (\<mu>, \<rho>)" by auto
       from in_lookup show "< (\<mu>, \<rho>) , V x > \<rightarrow> < (\<mu>, \<rho>) , Inr (SLoc xl, k) >" by (rule EVar)
     qed
   qed
@@ -107,13 +117,13 @@ next
         and not_in_lookup: "x \<notin> Map.dom \<mu>" by auto
   then show ?case
   proof -
-    show "\<exists>\<mu>' \<rho>' \<L>'. ((\<Gamma> \<union> {(x, f (empty, t))}) \<leftrightarrow> (\<mu>', \<rho>')) \<and> 
+    show "\<exists>\<mu>' \<rho>' \<L>'. ((\<Gamma>(x \<mapsto> f(empty, t))) \<leftrightarrow> (\<mu>', \<rho>')) \<and> 
                      < (\<mu>, \<rho>) , var x : t > \<rightarrow> < (\<mu>', \<rho>') , \<L>' >"
     proof(rule exI[where x = "\<mu>(x \<mapsto> (l, SLoc l))"],
           rule exI[where x = "\<rho>(l \<mapsto> (t, emptyVal t))"],
           rule exI[where x = "Inr (SLoc l, SLoc l)"],
           rule conjI)
-      from env_compat show "(\<Gamma> \<union> {(x, f (empty, t))}) \<leftrightarrow> (\<mu>(x \<mapsto> (l, SLoc l)), \<rho>(l \<mapsto> (t, emptyVal t)))"
+      from env_compat show "(\<Gamma>(x \<mapsto> f (empty, t))) \<leftrightarrow> (\<mu>(x \<mapsto> (l, SLoc l)), \<rho>(l \<mapsto> (t, emptyVal t)))"
         by auto
       from not_in_lookup and has_loc
       show "< (\<mu>, \<rho>) , var x : t > \<rightarrow> < (\<mu>(x \<mapsto> (l, SLoc l)), \<rho>(l \<mapsto> (t, emptyVal t))) , Inr (SLoc l, SLoc l) >"
